Weidenbach_Book/IsaSAT/IsaSAT_Setup2_LLVM.thy
@@ -127,10 +127,93 @@ global_interpretation units_since_last_GC: read_stats_param_adder0 where
     split: isasat_int.splits)
   subgoal by (auto simp: units_since_last_GC_st_code_def)
   done
-thm get_GC_units_opt_def
-find_theorems opts_GC_units_lim RETURN
-(*opts_GC_units_lim opts_rel_GC_units_lim_code*)
-lemmas [sepref_fr_rules] =
+
+definition get_GC_units_opt_code :: \<open>twl_st_wll_trail_fast2 \<Rightarrow> _\<close> where
+  \<open>get_GC_units_opt_code = read_opts_wl_heur_code opts_rel_GC_units_lim_code\<close>
+
+global_interpretation opts_GC_units_lim: read_opts_param_adder0 where
+  f' = \<open>RETURN o opts_GC_units_lim\<close> and
+  f = opts_rel_GC_units_lim_code and
+  x_assn = word_assn and
+  P = \<open>\<lambda>_. True\<close>
+  rewrites \<open>read_opts_wl_heur (RETURN o opts_GC_units_lim) = RETURN o get_GC_units_opt\<close> and
+    \<open>read_opts_wl_heur_code opts_rel_GC_units_lim_code = get_GC_units_opt_code\<close>
+  apply unfold_locales
+  apply (rule opts_refine)
+  subgoal by (auto simp: read_opts_wl_heur_def get_GC_units_opt_def intro!: ext
+    split: isasat_int.splits)
+  subgoal by (auto simp: get_GC_units_opt_code_def)
+  done
+
+definition isasat_length_trail_st_code :: \<open>twl_st_wll_trail_fast2 \<Rightarrow> _\<close> where
+  \<open>isasat_length_trail_st_code = read_trail_wl_heur_code isa_length_trail_fast_code\<close>
+
+global_interpretation trail_length: read_trail_param_adder0 where
+  f' = \<open>RETURN o isa_length_trail\<close> and
+  f = isa_length_trail_fast_code and
+  x_assn = sint64_nat_assn and
+  P = \<open>\<lambda>_. True\<close>
+  rewrites  \<open>read_trail_wl_heur (RETURN o isa_length_trail) = RETURN o isasat_length_trail_st\<close> and
+    \<open>read_trail_wl_heur_code isa_length_trail_fast_code = isasat_length_trail_st_code\<close>
+  apply unfold_locales
+  apply (rule isa_length_trail_fast_code.refine)
+  subgoal by (auto simp: isa_length_trail_def read_trail_wl_heur_def isasat_length_trail_st_def
+    intro!: ext split: isasat_int.splits)
+  subgoal by (auto simp: isasat_length_trail_st_code_def)
+  done
+
+term get_pos_of_level_in_trail_imp
+lemma get_pos_of_level_in_trail_imp_alt_def:
+  \<open>get_pos_of_level_in_trail_imp = (\<lambda>S C. do {k \<leftarrow> get_pos_of_level_in_trail_imp S C; RETURN k})\<close>
+  by auto
+
+sepref_def get_pos_of_level_in_trail_imp_code
+  is \<open>uncurry get_pos_of_level_in_trail_imp\<close>
+  :: \<open>trail_pol_fast_assn\<^sup>k *\<^sub>a uint32_nat_assn\<^sup>k  \<rightarrow>\<^sub>a sint64_nat_assn\<close>
+  supply [[goals_limit=1]]
+  apply (subst get_pos_of_level_in_trail_imp_alt_def)
+  apply (rewrite in \<open>_\<close> eta_expand[where f = RETURN])
+  apply (rewrite in \<open>RETURN \<hole>\<close> annot_unat_snat_upcast[where 'l=64])
+  by sepref
+
+definition get_pos_of_level_in_trail_imp_st_code :: \<open>twl_st_wll_trail_fast2 \<Rightarrow> _\<close> where
+  \<open>get_pos_of_level_in_trail_imp_st_code = (\<lambda>N C. read_trail_wl_heur_code (\<lambda>c. get_pos_of_level_in_trail_imp_code c C) N)\<close>
+
+global_interpretation pos_of_level_in_trail: read_trail_param_adder where
+  R = \<open>unat_rel' TYPE(32)\<close> and
+  f' = \<open>\<lambda>M c. get_pos_of_level_in_trail_imp c M\<close> and
+  f = \<open>\<lambda>M c. get_pos_of_level_in_trail_imp_code c M\<close> and
+  x_assn = sint64_nat_assn and
+  P = \<open>\<lambda>_ _. True\<close>
+  rewrites  \<open>(\<lambda>N C'. read_trail_wl_heur (\<lambda>c. get_pos_of_level_in_trail_imp c C') N) = get_pos_of_level_in_trail_imp_st\<close> and
+    \<open>(\<lambda>N C. read_trail_wl_heur_code (\<lambda>c. get_pos_of_level_in_trail_imp_code c C) N) = get_pos_of_level_in_trail_imp_st_code\<close>
+  apply unfold_locales
+  apply (rule remove_pure_parameter2[where f' =  \<open>get_pos_of_level_in_trail_imp\<close> and f =  \<open>get_pos_of_level_in_trail_imp_code\<close>])
+  apply (subst lambda_comp_true)+
+  apply (rule get_pos_of_level_in_trail_imp_code.refine, assumption)
+  subgoal by (auto simp: get_pos_of_level_in_trail_imp_st_def read_trail_wl_heur_def
+    intro!: ext split: isasat_int.splits)
+  subgoal by (auto simp: get_pos_of_level_in_trail_imp_st_code_def)
+  done
+
+definition get_global_conflict_count_impl :: \<open>twl_st_wll_trail_fast2 \<Rightarrow> _\<close> where
+   \<open>get_global_conflict_count_impl = read_stats_wl_heur_code stats_conflicts_stats_impl\<close>
+
+global_interpretation stats_conflict: read_stats_param_adder0 where
+  f' = \<open>RETURN o stats_conflicts\<close> and
+  f = stats_conflicts_stats_impl and
+  x_assn = word_assn and
+  P = \<open>\<lambda>_. True\<close>
+  rewrites \<open>read_stats_wl_heur (RETURN o stats_conflicts) = RETURN o get_global_conflict_count\<close> and
+    \<open>read_stats_wl_heur_code stats_conflicts_stats_impl = get_global_conflict_count_impl\<close>
+  apply unfold_locales
+  apply (rule stats_refine; assumption)
+  subgoal by (auto simp: read_stats_wl_heur_def stats_conflicts_def get_global_conflict_count_def intro!: ext
+    split: isasat_int.splits)
+  subgoal by (auto simp: get_global_conflict_count_impl_def)
+  done
+
+lemmas [unfolded lambda_comp_true, sepref_fr_rules] =
   opts_restart.refine[unfolded]
   opts_reduce.refine[unfolded]
   opts_unbounded_mode.refine
@@ -138,7 +221,14 @@ lemmas [sepref_fr_rules] =
   opts_restart_coeff1.refine
   opts_restart_coeff2.refine
   units_since_last_GC.refine
-  units_since_last_GC.refine
+  opts_GC_units_lim.refine
+  trail_length.refine
+  pos_of_level_in_trail.refine
+  stats_conflict.refine
+
+sepref_register opts_reduction_st opts_restart_st opts_restart_coeff2_st opts_restart_coeff1_st
+    opts_minimum_between_restart_st opts_unbounded_mode_st get_GC_units_opt units_since_last_GC_st
+    isasat_length_trail_st get_pos_of_level_in_trail_imp_st
 
 lemmas [unfolded inline_direct_return_node_case, llvm_code] =
   opts_restart_st_fast_code_def[unfolded read_opts_wl_heur_code_def]
@@ -148,12 +238,34 @@ lemmas [unfolded inline_direct_return_node_case, llvm_code] =
   opts_restart_coeff1_st_fast_code_def[unfolded read_opts_wl_heur_code_def]
   opts_restart_coeff2_st_fast_code_def[unfolded read_opts_wl_heur_code_def]
   units_since_last_GC_st_code_def[unfolded read_stats_wl_heur_def]
+  get_GC_units_opt_code_def[unfolded read_opts_wl_heur_code_def]
+  isasat_length_trail_st_code_def[unfolded read_trail_wl_heur_code_def]
+  get_pos_of_level_in_trail_imp_st_code_def[unfolded read_trail_wl_heur_code_def]
+  get_global_conflict_count_impl_def[unfolded read_stats_wl_heur_code_def]
 
 named_theorems state_extractors \<open>Definition of all functions modifying the state\<close>
 lemmas [state_extractors] =
+  extract_trail_wl_heur_def
+  extract_arena_wl_heur_def
+  extract_conflict_wl_heur_def
+  extract_watchlist_wl_heur_def
   extract_stats_wl_heur_def
+  extract_heur_wl_heur_def
+  extract_lcount_wl_heur_def
+  isasat_state_ops.remove_trail_wl_heur_def
+  isasat_state_ops.remove_arena_wl_heur_def
+  isasat_state_ops.remove_conflict_wl_heur_def
+  isasat_state_ops.remove_watchlist_wl_heur_def
   isasat_state_ops.remove_stats_wl_heur_def
+  isasat_state_ops.remove_heur_wl_heur_def
+  isasat_state_ops.remove_lcount_wl_heur_def
+  update_trail_wl_heur_def
+  update_arena_wl_heur_def
+  update_conflict_wl_heur_def
+  update_watchlist_wl_heur_def
   update_stats_wl_heur_def
+  update_heur_wl_heur_def
+  update_lcount_wl_heur_def
 
 sepref_register reset_units_since_last_GC
 
@@ -173,132 +285,167 @@ sepref_def reset_units_since_last_GC_st_code
   unfolding reset_units_since_last_GC_st_alt_def
   by sepref
 
+lemma mop_isasat_length_trail_st_alt_def:
+  \<open>mop_isasat_length_trail_st S = do {
+    ASSERT(isa_length_trail_pre (get_trail_wl_heur S));
+    RETURN (isasat_length_trail_st S)
+  }\<close>
+  unfolding isasat_length_trail_st_def mop_isasat_length_trail_st_def
+  by auto
 
-experiment
-begin
-export_llvm opts_reduction_st_fast_code opts_restart_st_fast_code opts_unbounded_mode_st_fast_code
-  opts_minimum_between_restart_st_fast_code
-end
-
-sepref_def get_GC_units_opt_code
-  is \<open>RETURN o get_GC_units_opt\<close>
-  :: \<open>isasat_bounded_assn\<^sup>k \<rightarrow>\<^sub>a word_assn\<close>
-  supply [[goals_limit=1]]
-  unfolding get_GC_units_opt_alt_def
-    isasat_bounded_assn_def fold_tuple_optimizations
-  by sepref
-
-sepref_register opts_reduction_st opts_restart_st opts_restart_coeff2_st opts_restart_coeff1_st
-    opts_minimum_between_restart_st opts_unbounded_mode_st get_GC_units_opt units_since_last_GC_st
-
-sepref_register isasat_length_trail_st
-
-sepref_def isasat_length_trail_st_code
-  is \<open>RETURN o isasat_length_trail_st\<close>
-  :: \<open>[isa_length_trail_pre o get_trail_wl_heur]\<^sub>a isasat_bounded_assn\<^sup>k  \<rightarrow> sint64_nat_assn\<close>
-  supply [[goals_limit=1]]
-  unfolding isasat_length_trail_st_alt_def isasat_bounded_assn_def
-  by sepref
 
 sepref_def mop_isasat_length_trail_st_code
   is \<open>mop_isasat_length_trail_st\<close>
   :: \<open>isasat_bounded_assn\<^sup>k  \<rightarrow>\<^sub>a sint64_nat_assn\<close>
   supply [[goals_limit=1]]
-  unfolding mop_isasat_length_trail_st_alt_def isasat_bounded_assn_def
+  unfolding mop_isasat_length_trail_st_alt_def
   by sepref
 
-sepref_register get_pos_of_level_in_trail_imp_st
 
-sepref_def get_pos_of_level_in_trail_imp_st_code
-  is \<open>uncurry get_pos_of_level_in_trail_imp_st\<close>
-  :: \<open>isasat_bounded_assn\<^sup>k *\<^sub>a uint32_nat_assn\<^sup>k  \<rightarrow>\<^sub>a sint64_nat_assn\<close>
-  supply [[goals_limit=1]]
-  unfolding get_pos_of_level_in_trail_imp_alt_def isasat_bounded_assn_def
-  apply (rewrite in \<open>_\<close> eta_expand[where f = RETURN])
-  apply (rewrite in \<open>RETURN \<hole>\<close> annot_unat_snat_upcast[where 'l=64])
-  by sepref
+definition arena_status_st where
+  \<open>arena_status_st = (\<lambda>S. arena_status (get_clauses_wl_heur S))\<close>
 
-sepref_def clause_not_marked_to_delete_heur_fast_code
-  is \<open>uncurry (RETURN oo clause_not_marked_to_delete_heur)\<close>
-  :: \<open>[clause_not_marked_to_delete_heur_pre]\<^sub>a isasat_bounded_assn\<^sup>k *\<^sub>a sint64_nat_assn\<^sup>k \<rightarrow> bool1_assn\<close>
-  supply [[goals_limit=1]]
-  unfolding clause_not_marked_to_delete_heur_alt_def isasat_bounded_assn_def
-     clause_not_marked_to_delete_heur_pre_def
-  by sepref
+definition arena_status_st_impl where
+  \<open>arena_status_st_impl = (\<lambda>S C'. read_arena_wl_heur_code (\<lambda>N. arena_status_impl N C') S)\<close>
 
-sepref_def mop_clause_not_marked_to_delete_heur_impl
-  is \<open>uncurry mop_clause_not_marked_to_delete_heur\<close>
-  :: \<open>isasat_bounded_assn\<^sup>k *\<^sub>a sint64_nat_assn\<^sup>k \<rightarrow>\<^sub>a bool1_assn\<close>
-  unfolding mop_clause_not_marked_to_delete_heur_alt_def
-    clause_not_marked_to_delete_heur_pre_def  prod.case isasat_bounded_assn_def
-  by sepref
+global_interpretation arena_is_valid: read_arena_param_adder where
+  R = \<open>snat_rel' TYPE(64)\<close> and
+  f = \<open>\<lambda>C N. arena_status_impl N C\<close> and
+  f' = \<open>(\<lambda>C' N.  (RETURN oo arena_status) N C')\<close> and
+  x_assn = status_impl_assn and
+  P = \<open>(\<lambda>C S. arena_is_valid_clause_vdom S C)\<close>
+  rewrites \<open>(\<lambda>S C'. read_arena_wl_heur (\<lambda>N.  (RETURN oo arena_status) N C') S) = RETURN oo arena_status_st\<close> and
+  \<open>(\<lambda>S C'. read_arena_wl_heur_code (\<lambda>N. arena_status_impl N C') S) = arena_status_st_impl\<close> and
+  \<open>arena_is_valid.mop = mop_arena_status_st\<close>
+  apply unfold_locales
+  apply (rule remove_pure_parameter2[where f =  \<open> \<lambda>N. arena_status_impl N\<close> and f' =  \<open>\<lambda>N C. (RETURN oo arena_status) N C\<close>])
+  apply (rule arena_status_impl.refine, assumption)
+  subgoal by (auto simp: mop_arena_status_st_def read_arena_wl_heur_def arena_status_st_def
+    intro!: ext split: isasat_int.splits)
+  subgoal by (auto simp: arena_status_st_impl_def)
+  subgoal by (auto simp: read_arena_param_adder_ops.mop_def mop_arena_status_st_def mop_arena_status_def read_arena_wl_heur_def arena_status_st_def
+    intro!: ext split: isasat_int.splits)
+  done
 
-sepref_def mop_arena_lbd_st_impl
-  is \<open>uncurry mop_arena_lbd_st\<close>
-  :: \<open>isasat_bounded_assn\<^sup>k *\<^sub>a sint64_nat_assn\<^sup>k \<rightarrow>\<^sub>a uint32_nat_assn\<close>
-  supply [[goals_limit=1]]
-  unfolding mop_arena_lbd_st_alt_def isasat_bounded_assn_def
-  by sepref
+lemmas [sepref_fr_rules] = arena_is_valid.mop_refine
 
 sepref_def mop_arena_status_st_impl
   is \<open>uncurry mop_arena_status_st\<close>
   :: \<open>isasat_bounded_assn\<^sup>k *\<^sub>a sint64_nat_assn\<^sup>k \<rightarrow>\<^sub>a status_impl_assn\<close>
   supply [[goals_limit=1]]
-  unfolding mop_arena_status_st_alt_def isasat_bounded_assn_def
   by sepref
 
-sepref_def mop_marked_as_used_st_impl
-  is \<open>uncurry mop_marked_as_used_st\<close>
-  :: \<open>isasat_bounded_assn\<^sup>k *\<^sub>a sint64_nat_assn\<^sup>k \<rightarrow>\<^sub>a unat_assn' TYPE(2)\<close>
-  supply [[goals_limit=1]]
-  unfolding mop_marked_as_used_st_alt_def isasat_bounded_assn_def
+definition arena_length_st_impl :: \<open>twl_st_wll_trail_fast2 \<Rightarrow> _\<close> where
+  \<open>arena_length_st_impl = (\<lambda>S C'. read_arena_wl_heur_code (\<lambda>N. arena_length_impl N C') S)\<close>
+
+global_interpretation arena_length_clause: read_arena_param_adder where
+  R = \<open>snat_rel' TYPE(64)\<close> and
+  f = \<open>\<lambda>C N. arena_length_impl N C\<close> and
+  f' = \<open>(\<lambda>C' N.  (RETURN oo arena_length) N C')\<close> and
+  x_assn = sint64_nat_assn and
+  P = \<open>(\<lambda>C S. arena_is_valid_clause_idx S C)\<close>
+  rewrites \<open>(\<lambda>S C'. read_arena_wl_heur (\<lambda>N.  (RETURN oo arena_status) N C') S) = RETURN oo arena_status_st\<close> and
+  \<open>(\<lambda>S C'. read_arena_wl_heur_code (\<lambda>N. arena_length_impl N C') S) = arena_length_st_impl\<close> and
+  \<open>arena_length_clause.mop = mop_arena_length_st\<close>
+  apply unfold_locales
+  apply (rule remove_pure_parameter2[where f =  \<open> \<lambda>N. arena_length_impl N\<close> and f' =  \<open>\<lambda>N C. (RETURN oo arena_length) N C\<close>])
+  apply (rule arena_length_impl.refine, assumption)
+  subgoal by (auto simp: mop_arena_status_st_def read_arena_wl_heur_def arena_status_st_def
+    intro!: ext split: isasat_int.splits)
+  subgoal by (auto simp: arena_length_st_impl_def)
+  subgoal
+    by (auto simp: read_arena_param_adder_ops.mop_def mop_arena_length_st_def mop_arena_length_def read_arena_wl_heur_def
+      split: isasat_int.splits intro!: ext)
+  done
+
+lemmas [sepref_fr_rules] = arena_length_clause.mop_refine
+lemmas [unfolded inline_direct_return_node_case, llvm_code] = arena_length_st_impl_def[unfolded read_arena_wl_heur_code_def]
+  arena_status_st_impl_def[unfolded read_arena_wl_heur_code_def]
+
+sepref_definition arena_full_length_impl
+  is \<open>RETURN o length\<close>
+  :: \<open>arena_fast_assn\<^sup>k \<rightarrow>\<^sub>a sint64_nat_assn\<close>
   by sepref
 
-sepref_def mop_arena_length_st_impl
-  is \<open>uncurry mop_arena_length_st\<close>
-  :: \<open>isasat_bounded_assn\<^sup>k *\<^sub>a sint64_nat_assn\<^sup>k \<rightarrow>\<^sub>a sint64_nat_assn\<close>
-  supply [[goals_limit=1]]
-  unfolding mop_arena_length_st_alt_def isasat_bounded_assn_def
-  by sepref
+definition full_arena_length_st_impl :: \<open>twl_st_wll_trail_fast2 \<Rightarrow> _\<close> where
+  \<open>full_arena_length_st_impl = read_arena_wl_heur_code  (arena_full_length_impl)\<close>
 
-sepref_register incr_wasted_st full_arena_length_st wasted_bytes_st
+global_interpretation arena_full_length: read_arena_param_adder0 where
+  f = \<open>arena_full_length_impl\<close> and
+  f' = \<open>(RETURN o length)\<close> and
+  x_assn = sint64_nat_assn and
+  P = \<open>(\<lambda>_. True)\<close>
+  rewrites \<open>read_arena_wl_heur (RETURN o length) = RETURN o full_arena_length_st\<close> and
+    \<open>read_arena_wl_heur_code  (arena_full_length_impl) = full_arena_length_st_impl\<close>
+  apply unfold_locales
+  apply (rule arena_full_length_impl.refine)
+  subgoal by (auto simp: mop_arena_status_st_def read_arena_wl_heur_def full_arena_length_st_def
+    intro!: ext split: isasat_int.splits)
+  subgoal by (auto simp: full_arena_length_st_impl_def)
+  done
+
+lemma incr_wasted_st_alt_def:
+  \<open>incr_wasted_st = (\<lambda>waste S. do{
+  let (heur, S) = extract_heur_wl_heur S in
+  let heur = incr_wasted waste heur in
+  let S = update_heur_wl_heur heur S in S
+  })\<close>
+    by (auto simp: incr_wasted_st_def state_extractors intro!: ext split: isasat_int.splits)
+
 sepref_def incr_wasted_st_impl
   is \<open>uncurry (RETURN oo incr_wasted_st)\<close>
   :: \<open>word64_assn\<^sup>k *\<^sub>a isasat_bounded_assn\<^sup>d \<rightarrow>\<^sub>a isasat_bounded_assn\<close>
   supply[[goals_limit=1]]
-  unfolding incr_wasted_st_def
-    isasat_bounded_assn_def fold_tuple_optimizations
+  unfolding incr_wasted_st_alt_def
   by sepref
 
-sepref_def full_arena_length_st_impl
-  is \<open>RETURN o full_arena_length_st\<close>
-  :: \<open>isasat_bounded_assn\<^sup>k \<rightarrow>\<^sub>a sint64_nat_assn\<close>
-  unfolding full_arena_length_st_def isasat_bounded_assn_def
-  by sepref
+lemma id_clvls_assn: \<open>(Mreturn, RETURN) \<in> (uint32_nat_assn)\<^sup>k \<rightarrow>\<^sub>a uint32_nat_assn\<close>
+  by sepref_to_hoare vcg
 
-sepref_register get_global_conflict_count
-sepref_def get_global_conflict_count_impl
-  is \<open>RETURN o get_global_conflict_count\<close>
-  :: \<open>isasat_bounded_assn\<^sup>k \<rightarrow>\<^sub>a word_assn\<close>
-  unfolding get_global_conflict_count_alt_def isasat_bounded_assn_def
-  by sepref
+definition get_count_max_lvls_heur_impl :: \<open>twl_st_wll_trail_fast2 \<Rightarrow> _\<close> where
+  \<open>get_count_max_lvls_heur_impl = read_clvls_wl_heur_code  (Mreturn)\<close>
 
-sepref_def get_count_max_lvls_heur_impl
-  is \<open>RETURN o get_count_max_lvls_heur\<close>
-  :: \<open>isasat_bounded_assn\<^sup>k \<rightarrow>\<^sub>a uint32_nat_assn\<close>
-  unfolding get_count_max_lvls_heur_def isasat_bounded_assn_def
-  by sepref
+global_interpretation get_count_max_lvls: read_clvls_param_adder0 where
+  f = \<open>Mreturn\<close> and
+  f' = \<open>(RETURN)\<close> and
+  x_assn = uint32_nat_assn and
+  P = \<open>(\<lambda>_. True)\<close>
+  rewrites \<open>read_clvls_wl_heur (RETURN) = RETURN o get_count_max_lvls_heur\<close> and
+    \<open>read_clvls_wl_heur_code  (Mreturn) = get_count_max_lvls_heur_impl\<close>
+  apply unfold_locales
+  apply (rule id_clvls_assn)
+  subgoal by (auto simp: read_clvls_wl_heur_def get_count_max_lvls_heur_def
+    intro!: ext split: isasat_int.splits)
+  subgoal by (auto simp: get_count_max_lvls_heur_impl_def)
+  done
+
+
+lemmas [sepref_fr_rules] = arena_full_length.refine get_count_max_lvls.refine
+lemmas [unfolded inline_direct_return_node_case, llvm_code] = full_arena_length_st_impl_def[unfolded read_arena_wl_heur_code_def]
+  arena_full_length_impl_def
+   get_count_max_lvls_heur_impl_def[unfolded read_clvls_wl_heur_code_def]
+
+lemma clss_size_resetUS0_st_alt_def:
+  \<open>clss_size_resetUS0_st S =
+  (let (stats, S) = extract_lcount_wl_heur S in
+  let stats = clss_size_resetUS0 stats in
+  let S = update_lcount_wl_heur stats S in S
+  )\<close>
+  by (auto simp: clss_size_resetUS0_st_def state_extractors
+    split: isasat_int.splits)
 
 sepref_def clss_size_resetUS0_st
   is \<open>RETURN o clss_size_resetUS0_st\<close>
   :: \<open>isasat_bounded_assn\<^sup>d \<rightarrow>\<^sub>a isasat_bounded_assn\<close>
-  unfolding fold_tuple_optimizations isasat_bounded_assn_def clss_size_resetUS0_st_alt_def
+  unfolding clss_size_resetUS0_st_alt_def
   by sepref
 
-sepref_def length_clauses_heur_impl
-  is \<open>RETURN o length_clauses_heur\<close>
-  :: \<open>isasat_bounded_assn\<^sup>k \<rightarrow>\<^sub>a sint64_nat_assn\<close>
-  unfolding length_clauses_heur_alt_def isasat_bounded_assn_def
-  by sepref
+experiment
+begin
+export_llvm opts_reduction_st_fast_code opts_restart_st_fast_code opts_unbounded_mode_st_fast_code
+  opts_minimum_between_restart_st_fast_code mop_arena_status_st_impl full_arena_length_st_impl
+  get_global_conflict_count_impl get_count_max_lvls_heur_impl clss_size_resetUS0_st
+end
+
 
 end
